trying to refactor sums to make generic

code/mlkem/Hacl.Spec.MLkem.Sums.fst
@@ -7,202 +7,205 @@ unfold let max = FStar.Math.Lib.max
 open Lib.IntTypes
 open Lib.Sequence
 open Lib.NatMod
-open Hacl.Spec.MLkem.Zq
 
-// sum_of_zqs is sum_{i=start}^{stop-1} f(i)
-let rec sum_of_zqs (start:int) (stop:int) (f:(i:int -> zq)): Tot zq (decreases stop - start) =
+// let a = 1 `add_mod #(3)` 2
+
+// sum_of_modint is sum_{i=start}^{stop-1} f(i)
+let rec sum_of_modint (#m:pos{m > 1}) (start:int) (stop:int) (f:(i:int -> nat_mod m)): Tot (nat_mod m) (decreases stop - start) =
   if start >= stop then 0
-  else f (stop - 1) +% (sum_of_zqs start (stop - 1) f)
+  else f (stop - 1) `add_mod #m` (sum_of_modint #m start (stop - 1) f)
 
 // Lemmas about sum
 
 #reset-options "--z3rlimit 10"
-let lemma_sum_none (start:int) (f:int -> zq) : Lemma
+let lemma_sum_none (#m:pos{m > 1}) (start:int) (f:int -> nat_mod m) : Lemma
   (requires True)
-  (ensures 0 == (sum_of_zqs start start f))
-  [SMTPat (sum_of_zqs start start f)]
+  (ensures 0 == (sum_of_modint #m start start f))
   =
   ()
 
 // f = g ==> sum f = sum g
-let rec sum_rewrite_lemma (start stop:int) (f g:int -> zq): Lemma
+let rec sum_rewrite_lemma (#m:pos{m > 1})  (start stop:int) (f g:int -> nat_mod m): Lemma
     (requires (forall (i:int).{:pattern (f i)} start <= i /\ i < stop ==> f i == g i))
-    (ensures (sum_of_zqs start stop f) == (sum_of_zqs start stop g))
+    (ensures (sum_of_modint #m start stop f) == (sum_of_modint #m start stop g))
     (decreases (stop - start))
-    [SMTPat (sum_of_zqs start stop f)] 
     =
   if start < stop then sum_rewrite_lemma start (stop - 1) f g
 
-let double_sum_rewrite_lemma (start1 stop1 start2 stop2:int) (f g:int -> int -> zq): Lemma 
+#reset-options "--z3rlimit 15 --fuel 1"
+let double_sum_rewrite_lemma (#m:pos{m > 1}) (start1 stop1 start2 stop2:int) (f g:int -> int -> nat_mod m): Lemma 
   (requires (forall (i j:int). start1 <= i /\ i < stop1 /\ start2 <= j /\ j < stop2 ==> f i j == g i j))
-  (ensures sum_of_zqs start1 stop1 (fun i -> sum_of_zqs start2 stop2 (fun j -> f i j)) 
-        == sum_of_zqs start1 stop1 (fun i -> sum_of_zqs start2 stop2 (fun j -> g i j))) =
-  let original_f = (fun i -> sum_of_zqs start2 stop2 (fun j -> f i j)) in 
-  let goal_f = (fun i -> sum_of_zqs start2 stop2 (fun j -> g i j)) in
+  (ensures sum_of_modint #m start1 stop1 (fun i -> sum_of_modint #m start2 stop2 (fun j -> f i j)) 
+        == sum_of_modint #m start1 stop1 (fun i -> sum_of_modint #m start2 stop2 (fun j -> g i j))) =
+  let original_f = (fun i -> sum_of_modint #m start2 stop2 (fun j -> f i j)) in 
+  let goal_f = (fun i -> sum_of_modint #m start2 stop2 (fun j -> g i j)) in
   let lemma_aux (i:int{start1 <= i /\ i < stop1}): Lemma (original_f i == goal_f i) = 
     sum_rewrite_lemma start2 stop2 (fun j -> f i j) (fun j -> g i j) in
   Classical.forall_intro lemma_aux;
   sum_rewrite_lemma start1 stop1 original_f goal_f
 
+#reset-options "--z3rlimit 15"
 // sum_{i=start}^{stop-1} a * f(i) = a * sum_{i=start}^{stop-1} f(i)
 // = a * sum_{i=start}^{stop-1} f'(i)
-let rec sum_mul_lemma (a:zq) (start stop:int) (f:int -> zq): Lemma
+let rec sum_mul_lemma (#m:pos{m > 1}) (a:nat_mod m) (start stop:int) (f:int -> nat_mod m): Lemma
     // (requires start <= stop)
-    (ensures mul_zq a (sum_of_zqs start stop f) == sum_of_zqs start stop (fun i -> mul_zq a (f i)))
-    (decreases (stop - start))
-    [SMTPat (sum_of_zqs start stop (fun i -> a %* (f i)))] =
+    (ensures a `mul_mod #m` (sum_of_modint #m start stop f) == sum_of_modint #m start stop (fun i -> a `mul_mod #m` (f i)))
+    (decreases (stop - start)) =
   if start < stop then (
     sum_mul_lemma a start (stop - 1) f;
     calc (==) {
-      mul_zq a (sum_of_zqs start stop f);
+      a `mul_mod #m` (sum_of_modint #m start stop f);
       (==) {}
-      a %* ((sum_of_zqs start (stop - 1) f) +% f (stop - 1));
-      (==) {lemma_mod_distributivity_add_right #q a (sum_of_zqs start (stop - 1) f) (f (stop - 1))}
-      (a %* (sum_of_zqs start (stop - 1) f)) +% (a %* f (stop - 1));
+      a `mul_mod #m` ((sum_of_modint #m start (stop - 1) f) `add_mod #m` f (stop - 1));
+      (==) {lemma_mod_distributivity_add_right #m a (sum_of_modint #m start (stop - 1) f) (f (stop - 1))}
+      (a `mul_mod #m` (sum_of_modint #m start (stop - 1) f)) `add_mod #m` (a `mul_mod #m` f (stop - 1));
     }
   )
 
-let double_sum_mul_lemma_ (start1 stop1 start2 stop2:int) (f_i:int -> zq) (f_j:int -> int -> zq) (i:int{i >= start1 && i < stop1}): Lemma 
-  (ensures (f_i i %* sum_of_zqs start2 stop2 (f_j i)) == sum_of_zqs start2 stop2 (fun j -> f_i i %* (f_j i) j)) =
+let double_sum_mul_lemma_ (#m:pos{m > 1}) (start1 stop1 start2 stop2:int) (f_i:int -> nat_mod m) (f_j:int -> int -> nat_mod m) (i:int{i >= start1 && i < stop1}): Lemma 
+  (ensures (f_i i `mul_mod #m` sum_of_modint #m start2 stop2 (f_j i)) == sum_of_modint #m start2 stop2 (fun j -> f_i i `mul_mod #m` (f_j i) j)) =
   sum_mul_lemma (f_i i) start2 stop2 (f_j i)
 
 
-let double_sum_mul_lemma (start1 stop1 start2 stop2:int) (f_i:int -> zq) (f_j:int -> int -> zq): Lemma 
-  (ensures sum_of_zqs start1 stop1 (fun i -> (f_i i %* sum_of_zqs start2 stop2 (f_j i))) 
-        == sum_of_zqs start1 stop1 (fun i -> sum_of_zqs start2 stop2 (fun j -> f_i i %* (f_j i) j))) =
-  let f = (fun i -> (f_i i %* sum_of_zqs start2 stop2 (f_j i))) in
-  let f' = (fun i -> sum_of_zqs start2 stop2 (fun j -> f_i i %* (f_j i) j)) in
+let double_sum_mul_lemma (#m:pos{m > 1}) (start1 stop1 start2 stop2:int) (f_i:int -> nat_mod m) (f_j:int -> int -> nat_mod m): Lemma 
+  (ensures sum_of_modint #m start1 stop1 (fun i -> (f_i i `mul_mod #m` sum_of_modint #m start2 stop2 (f_j i))) 
+        == sum_of_modint #m start1 stop1 (fun i -> sum_of_modint #m start2 stop2 (fun j -> f_i i `mul_mod #m` (f_j i) j))) =
+  let f = (fun i -> (f_i i `mul_mod #m` sum_of_modint #m start2 stop2 (f_j i))) in
+  let f' = (fun i -> sum_of_modint #m start2 stop2 (fun j -> f_i i `mul_mod #m` (f_j i) j)) in
   Classical.forall_intro (double_sum_mul_lemma_ start1 stop1 start2 stop2 f_i f_j);
   assert (forall (i:int).{:pattern (f i)} start1 <= i /\ i < stop1 ==> f i == f' i);
   sum_rewrite_lemma start1 stop1 f f'
 
-let unfold_sum (start stop:int) (f:int -> zq): Lemma 
+let unfold_sum (#m:pos{m > 1}) (start stop:int) (f:int -> nat_mod m): Lemma 
     (requires stop > start)
-    (ensures (sum_of_zqs start stop f) == ((sum_of_zqs start (stop-1) f) +% f (stop - 1))) = 
+    (ensures (sum_of_modint #m start stop f) == ((sum_of_modint #m start (stop-1) f) `add_mod #m` f (stop - 1))) = 
   ()
 
-let lemma_rearrange (a b c d:zq) : Lemma
-    (ensures a +% b +% c +% d == a +% c +% b +% d) =
-  lemma_add_mod_comm #q b c;
-  assert (b +% c == c +% b);
+let lemma_rearrange (#m:pos{m > 1}) (a b c d:nat_mod m) : Lemma
+    (ensures a `add_mod #m` b `add_mod #m` c `add_mod #m` d == a `add_mod #m` c `add_mod #m` b `add_mod #m` d) =
+  lemma_add_mod_comm #m b c;
+  assert (b `add_mod #m` c == c `add_mod #m` b);
   calc (==) {
-    a +% b +% c +% d;
-    (==) {lemma_add_mod_assoc #q a b c}
-    a +% (b +% c) +% d;
+    a `add_mod #m` b `add_mod #m` c `add_mod #m` d;
+    (==) {lemma_add_mod_assoc #m a b c}
+    a `add_mod #m` (b `add_mod #m` c) `add_mod #m` d;
     (==) {}
-    a +% (c +% b) +% d;
-    (==) {lemma_add_mod_assoc #q a c b}
-    a +% c +% b +% d;
+    a `add_mod #m` (c `add_mod #m` b) `add_mod #m` d;
+    (==) {lemma_add_mod_assoc #m a c b}
+    a `add_mod #m` c `add_mod #m` b `add_mod #m` d;
   }
 
-let lemma_mul_rearrange (a b c d:zq) : Lemma 
-  (ensures a %* b %* c %* d == c %* a %* b %* d) =
-  assert (b %* c == c %* b);
+let lemma_mul_rearrange (#m:pos{m > 1}) (a b c d:nat_mod m) : Lemma 
+  (ensures a `mul_mod #m` b `mul_mod #m` c `mul_mod #m` d == c `mul_mod #m` a `mul_mod #m` b `mul_mod #m` d) =
+  assert (b `mul_mod #m` c == c `mul_mod #m` b);
   calc (==) {
-    a %* b %* c %* d;
-    (==) {}
-    a %* (b %* c) %* d;
-    (==) {}
-    a %* c %* b %* d;
+    a `mul_mod #m` b `mul_mod #m` c `mul_mod #m` d;
+    (==) {lemma_mul_mod_assoc #m a b c}
+    a `mul_mod #m` (b `mul_mod #m` c) `mul_mod #m` d;
+    (==) {lemma_mul_mod_comm #m b c}
+    a `mul_mod #m` (c `mul_mod #m` b) `mul_mod #m` d;
+    (==) {lemma_mul_mod_assoc #m a c b}
+    a `mul_mod #m` c `mul_mod #m` b `mul_mod #m` d;
+    (==) {lemma_mul_mod_comm #m a c}
+    c `mul_mod #m` a `mul_mod #m` b `mul_mod #m` d;
   }
 
-let lemma_mul_assoc_big (a b c d:zq): Lemma 
-  (ensures a %* (b %* c %* d) == a %* b %* c %* d) =
+let lemma_mul_assoc_big (#m:pos{m > 1}) (a b c d:nat_mod m): Lemma 
+  (ensures a `mul_mod #m` (b `mul_mod #m` c `mul_mod #m` d) == a `mul_mod #m` b `mul_mod #m` c `mul_mod #m` d) =
   calc (==) {
-    a %* (b %* c %* d);
-    (==) {}
-    a %* (b %* (c %* d));
-    (==) {}
-    a %* b %* (c %* d);
+    a `mul_mod #m` (b `mul_mod #m` c `mul_mod #m` d);
+    (==) {lemma_mul_mod_assoc #m a (b `mul_mod #m` c) d}
+    (a `mul_mod #m` (b `mul_mod #m` c)) `mul_mod #m` d;
+    (==) {lemma_mul_mod_assoc #m a b c}
+    a `mul_mod #m` b `mul_mod #m` c `mul_mod #m` d;
   }
 
-let lemma_mul_assoc_bigger (a b c d e:zq): Lemma 
-  (ensures a %* (b %* c %* d %* e) == a %* b %* c %* d %* e) =
-  lemma_mul_assoc_big b c d e;
-  assert (b %* c %* d %* e == b %* (c %* d %* e));
+let lemma_mul_assoc_bigger (#m:pos{m > 1}) (a b c d e:nat_mod m): 
+  Lemma 
+    (a `mul_mod #m` (b `mul_mod #m` c `mul_mod #m` d `mul_mod #m` e) 
+  == a `mul_mod #m` b `mul_mod #m` c `mul_mod #m` d `mul_mod #m` e) 
+=
   calc (==) {
-    a %* (b %* c %* d %* e);
-    (==) {}
-    a %* (b %* (c %* d %* e));
-    (==) {}
-    a %* b %* (c %* d %* e);
-    (==) {}
-    a %* b %* (c %* (d %* e));
-    (==) {}
-    a %* b %* c %* (d %* e);
+    a `mul_mod #m` (b `mul_mod #m` c `mul_mod #m` d `mul_mod #m` e);
+    (==) {lemma_mul_mod_assoc #m a (b `mul_mod #m` c `mul_mod #m` d) e}
+    (a `mul_mod #m` (b `mul_mod #m` c `mul_mod #m` d)) `mul_mod #m` e;
+    (==) {lemma_mul_assoc_big #m a b c d}
+    (a `mul_mod #m` b `mul_mod #m` c `mul_mod #m` d) `mul_mod #m` e;
   }
 
-let rec distribute_sum_lemma (start stop:int) (f:int -> zq) (g:int -> zq): Lemma
-    (ensures sum_of_zqs start stop (fun i -> f i +% g i) == sum_of_zqs start stop f +% sum_of_zqs start stop g)
+#reset-options "--z3rlimit 15 --fuel 1 --split_queries always"
+let rec distribute_sum_lemma (#m:pos{m > 1}) (start stop:int) (f:int -> nat_mod m) (g:int -> nat_mod m): Lemma
+    (ensures sum_of_modint #m start stop (fun i -> f i `add_mod #m` g i) == sum_of_modint #m start stop f `add_mod #m` sum_of_modint #m start stop g)
     (decreases stop - start) =
   if start < stop then (
     distribute_sum_lemma start (stop - 1) f g;
     calc (==) {
-      sum_of_zqs start stop (fun i -> f i +% g i);
+      sum_of_modint #m start stop (fun i -> f i `add_mod #m` g i);
       (==) {}
-      sum_of_zqs start (stop-1) (fun i -> f i +% g i) +% (f (stop-1) +% g (stop-1));
-      (==) {lemma_add_mod_assoc #q (sum_of_zqs start (stop-1) (fun i -> f i +% g i)) (f (stop-1)) (g (stop-1))}
-      sum_of_zqs start (stop-1) (fun i -> f i +% g i) +% f (stop-1) +% g (stop-1);
+      sum_of_modint #m start (stop-1) (fun i -> f i `add_mod #m` g i) `add_mod #m` (f (stop-1) `add_mod #m` g (stop-1));
+      (==) {lemma_add_mod_assoc #m (sum_of_modint #m start (stop-1) (fun i -> f i `add_mod #m` g i)) (f (stop-1)) (g (stop-1))}
+      sum_of_modint #m start (stop-1) (fun i -> f i `add_mod #m` g i) `add_mod #m` f (stop-1) `add_mod #m` g (stop-1);
       (==) {}
-      sum_of_zqs start (stop-1) f +% sum_of_zqs start (stop-1) g +% f (stop-1) +% g (stop-1);
+      sum_of_modint #m start (stop-1) f `add_mod #m` sum_of_modint #m start (stop-1) g `add_mod #m` f (stop-1) `add_mod #m` g (stop-1);
     };
     calc (==) {
-      sum_of_zqs start stop f +% sum_of_zqs start stop g;
+      sum_of_modint #m start stop f `add_mod #m` sum_of_modint #m start stop g;
       (==) {}
-      (sum_of_zqs start (stop-1) f +% f (stop-1)) +% (sum_of_zqs start (stop-1) g +% g (stop-1));
-      (==) {lemma_add_mod_assoc #q (sum_of_zqs start (stop-1) f) (f (stop-1)) (sum_of_zqs start (stop-1) g +% g (stop-1))}
-      sum_of_zqs start (stop-1) f +% f (stop-1) +% (sum_of_zqs start (stop-1) g +% g (stop-1));
-      (==) {lemma_add_mod_assoc #q (sum_of_zqs start (stop-1) f +% f (stop-1)) (sum_of_zqs start (stop-1) g) (g (stop-1))}
-      sum_of_zqs start (stop-1) f +% f (stop-1) +% sum_of_zqs start (stop-1) g +% g (stop-1);
-      (==) { lemma_rearrange (sum_of_zqs start (stop-1) f) (f (stop-1)) (sum_of_zqs start (stop-1) g) (g (stop-1))}
-      sum_of_zqs start (stop-1) f +% sum_of_zqs start (stop-1) g +% f (stop-1) +% g (stop-1);
+      (sum_of_modint #m start (stop-1) f `add_mod #m` f (stop-1)) `add_mod #m` (sum_of_modint #m start (stop-1) g `add_mod #m` g (stop-1));
+      (==) {lemma_add_mod_assoc #m (sum_of_modint #m start (stop-1) f) (f (stop-1)) (sum_of_modint #m start (stop-1) g `add_mod #m` g (stop-1))}
+      sum_of_modint #m start (stop-1) f `add_mod #m` f (stop-1) `add_mod #m` (sum_of_modint #m start (stop-1) g `add_mod #m` g (stop-1));
+      (==) {lemma_add_mod_assoc #m (sum_of_modint #m start (stop-1) f `add_mod #m` f (stop-1)) (sum_of_modint #m start (stop-1) g) (g (stop-1))}
+      sum_of_modint #m start (stop-1) f `add_mod #m` f (stop-1) `add_mod #m` sum_of_modint #m start (stop-1) g `add_mod #m` g (stop-1);
+      (==) { lemma_rearrange (sum_of_modint #m start (stop-1) f) (f (stop-1)) (sum_of_modint #m start (stop-1) g) (g (stop-1))}
+      sum_of_modint #m start (stop-1) f `add_mod #m` sum_of_modint #m start (stop-1) g `add_mod #m` f (stop-1) `add_mod #m` g (stop-1);
     }
   )
 
-let unfold_double_sum_inner (start1 start2 stop1 stop2:int) (f:int -> int -> zq): Lemma 
+#reset-options "--z3rlimit 15"
+let unfold_double_sum_inner (#m:pos{m > 1}) (start1 start2 stop1 stop2:int) (f:int -> int -> nat_mod m): Lemma 
     (requires stop2 > start2)
-    (ensures sum_of_zqs start1 stop1 (fun i -> sum_of_zqs start2 stop2 (fun j -> f i j)) 
-         ==  sum_of_zqs start1 stop1 (fun i -> (sum_of_zqs start2 (stop2-1) (fun j -> f i j)) +% (f i (stop2-1)))) = 
-  let inner_f = (fun i -> sum_of_zqs start2 stop2 (fun j -> f i j)) in
-  let inner_f_unfolded = (fun i -> (sum_of_zqs start2 (stop2-1) (fun j -> f i j)) +% f i (stop2-1)) in
+    (ensures sum_of_modint #m start1 stop1 (fun i -> sum_of_modint #m start2 stop2 (fun j -> f i j)) 
+         ==  sum_of_modint #m start1 stop1 (fun i -> (sum_of_modint #m start2 (stop2-1) (fun j -> f i j)) `add_mod #m` (f i (stop2-1)))) = 
+  let inner_f = (fun i -> sum_of_modint #m start2 stop2 (fun j -> f i j)) in
+  let inner_f_unfolded = (fun i -> (sum_of_modint #m start2 (stop2-1) (fun j -> f i j)) `add_mod #m` f i (stop2-1)) in
   sum_rewrite_lemma start1 stop1 inner_f inner_f_unfolded
 
 // Unfolding a double sum should give us:
 // sum^n sum^m (f i j) = (sum^n-1 sum^m-1 (f i j)) + (sum^n-1 (f i m)) + (sum^m-1 (f n j)) + (f n m)
 // Call it sum^n sum^m (f i j) = A + B + C + D
-let unfold_double_sum (start1 start2 stop1 stop2:int) (f:int -> int -> zq): Lemma
+let unfold_double_sum (#m:pos{m > 1}) (start1 start2 stop1 stop2:int) (f:int -> int -> nat_mod m): Lemma
     (requires stop1 > start1 /\ stop2 > start2)
-    (ensures sum_of_zqs start1 stop1 (fun i -> sum_of_zqs start2 stop2 (fun j -> f i j)) 
-              ==  sum_of_zqs start1 (stop1-1) (fun i -> 
-                    (sum_of_zqs start2 (stop2-1) (fun j -> f i j)) +% (f i (stop2-1))) 
-                  +% (sum_of_zqs start1 (stop1-1) (fun j -> f (stop1-1) j)) 
-                  +% f (stop1-1) (stop2-1)) =
-  let a = sum_of_zqs start1 (stop1-1) (fun i -> sum_of_zqs start2 (stop2-1) (fun j -> f i j)) in
-  let b = sum_of_zqs start1 (stop1-1) (fun i -> f i (stop2-1)) in
-  let c = sum_of_zqs start1 (stop1-1) (fun j -> f (stop1-1) j) in
+    (ensures sum_of_modint #m start1 stop1 (fun i -> sum_of_modint #m start2 stop2 (fun j -> f i j)) 
+              ==  sum_of_modint #m start1 (stop1-1) (fun i -> 
+                    (sum_of_modint #m start2 (stop2-1) (fun j -> f i j)) `add_mod #m` (f i (stop2-1))) 
+                  `add_mod #m` (sum_of_modint #m start1 (stop1-1) (fun j -> f (stop1-1) j)) 
+                  `add_mod #m` f (stop1-1) (stop2-1)) =
+  let a = sum_of_modint #m start1 (stop1-1) (fun i -> sum_of_modint #m start2 (stop2-1) (fun j -> f i j)) in
+  let b = sum_of_modint #m start1 (stop1-1) (fun i -> f i (stop2-1)) in
+  let c = sum_of_modint #m start1 (stop1-1) (fun j -> f (stop1-1) j) in
   let d = f (stop1-1) (stop2-1) in
-  let initial_sum = sum_of_zqs start1 stop1 (fun i -> sum_of_zqs start2 stop2 (fun j -> f i j)) in
+  let initial_sum = sum_of_modint #m start1 stop1 (fun i -> sum_of_modint #m start2 stop2 (fun j -> f i j)) in
   unfold_double_sum_inner start1 start2 stop1 stop2 f;
-  let unfolded_inner_f = (fun i -> (sum_of_zqs start2 (stop2-1) (fun j -> f i j)) +% (f i (stop2-1))) in
-  assert (initial_sum == sum_of_zqs start1 stop1 (fun i -> unfolded_inner_f i));
+  let unfolded_inner_f = (fun i -> (sum_of_modint #m start2 (stop2-1) (fun j -> f i j)) `add_mod #m` (f i (stop2-1))) in
+  assert (initial_sum == sum_of_modint #m start1 stop1 (fun i -> unfolded_inner_f i));
   unfold_sum start1 stop1 unfolded_inner_f;
-  assert (initial_sum == sum_of_zqs start1 (stop1-1) (fun i -> unfolded_inner_f i) +% unfolded_inner_f (stop1-1));
-  let a_f = (fun i -> sum_of_zqs start2 (stop2-1) (fun j -> f i j)) in
+  assert (initial_sum == sum_of_modint #m start1 (stop1-1) (fun i -> unfolded_inner_f i) `add_mod #m` unfolded_inner_f (stop1-1));
+  let a_f = (fun i -> sum_of_modint #m start2 (stop2-1) (fun j -> f i j)) in
   let b_f = (fun i -> f i (stop2-1)) in
   distribute_sum_lemma start1 stop1 a_f b_f;
-  // assert (sum_of_zqs start1 (stop1-1));
-  // assert (initial_sum == sum_of_zqs start1 (stop1-1) (fun i -> sum_of_zqs start2 (stop2-1) (fun j -> f i j)) +% sum_of_zqs start1 (stop1-1) (fun i -> f i (stop2-1)) +% unfolded_inner_f (stop1-1));
+  // assert (sum_of_modint #m start1 (stop1-1));
+  // assert (initial_sum == sum_of_modint #m start1 (stop1-1) (fun i -> sum_of_modint #m start2 (stop2-1) (fun j -> f i j)) `add_mod #m` sum_of_modint #m start1 (stop1-1) (fun i -> f i (stop2-1)) `add_mod #m` unfolded_inner_f (stop1-1));
   admit()
-  // assert (sum_of_zqs start1 (stop1-1) (fun i -> unfolded_inner_f i)
-  //      == sum_of_zqs start1 (stop1-1) (fun i -> (sum_of_zqs start2 (stop2-1) (fun j -> f i j))) +%
-  //           sum_of_zqs start1 (stop1-1) (fun i -> f i (stop2-1)));
+  // assert (sum_of_modint #m start1 (stop1-1) (fun i -> unfolded_inner_f i)
+  //      == sum_of_modint #m start1 (stop1-1) (fun i -> (sum_of_modint #m start2 (stop2-1) (fun j -> f i j))) `add_mod #m`
+  //           sum_of_modint #m start1 (stop1-1) (fun i -> f i (stop2-1)));
   // admit()
   // admit()
 
 
-let rec swap_sum_order (start1 stop1 start2 stop2:int) (f:int -> int -> zq): Lemma
+let rec swap_sum_order (#m:pos{m > 1}) (start1 stop1 start2 stop2:int) (f:int -> int -> nat_mod m): Lemma
     // (requires True)
-    (ensures sum_of_zqs start1 stop1 (fun i -> sum_of_zqs start2 stop2 (fun j -> f i j)) 
-          == sum_of_zqs start2 stop2 (fun j -> sum_of_zqs start1 stop1 (fun i -> f i j)))
+    (ensures sum_of_modint #m start1 stop1 (fun i -> sum_of_modint #m start2 stop2 (fun j -> f i j)) 
+          == sum_of_modint #m start2 stop2 (fun j -> sum_of_modint #m start1 stop1 (fun i -> f i j)))
     (decreases (stop1 - start1)) =
   admit()
